pulse/lib/pulse/core/PulseCore.IndirectionTheoryActions.fst
@@ -25,11 +25,10 @@ let pm_sep_laws () : squash (
   )
   
 let pm_sep : PulseCore.HeapSig.separable pulse_mem = PM.pulse_heap_sig.sep
-let pm_core_of (m:pulse_mem) : pulse_core_mem = PM.pulse_heap_sig.sep.core_of m
 
 // 
-let split_mem3 (pp qq rr:slprop) (s:erased core_mem { interp (pp `star` qq `star` rr) s })
-: res:(erased core_mem & erased core_mem & erased core_mem) {
+let split_mem3 (pp qq rr:slprop) (s:erased mem { interp (pp `star` qq `star` rr) s })
+: res:(erased mem & erased mem & erased mem) {
     let l, m, r = res in
     // disjoint l m /\
     disjoint m r /\
@@ -41,7 +40,7 @@ let split_mem3 (pp qq rr:slprop) (s:erased core_mem { interp (pp `star` qq `star
 }
 = sep_laws();
   let m1, m2 = split_mem pp (qq `star` rr) s in
-  let lr :erased (erased core_mem & erased core_mem) = hide (split_mem qq rr m2) in
+  let lr :erased (erased mem & erased mem) = hide (split_mem qq rr m2) in
   let l, m, r = m1, fst <| reveal lr, snd <| reveal lr in
   l, m, r
 
@@ -53,11 +52,10 @@ let pin_frame (p:pm_slprop) (frame:slprop)
     Lemma 
       (requires PM.interp (q `PM.star` frame') m')
       (ensures interpret (lift q `star` frame) { w with pulse_mem = m'}))
-= let c = core_of w in
-  let { pulse_mem; istore } = w in
-  let m0, m1 = split_mem (lift p) frame c in
-  star_equiv (lift p) frame c;
-  let fr (pm:pulse_core_mem)  
+= let { pulse_mem; istore } = w in
+  let m0, m1 = split_mem (lift p) frame w in
+  star_equiv (lift p) frame w;
+  let fr (pm:IndirectionTheorySep.pulse_mem)  
     : prop
     = interp frame { pulse_mem=pm; istore=m1.istore }
   in
@@ -82,25 +80,25 @@ let pin_frame (p:pm_slprop) (frame:slprop)
   PM.pulse_heap_sig.interp_as fr;
   assert (PM.pulse_heap_sig.interp frame' m1.pulse_mem);
   assert (pm_sep.disjoint m0.pulse_mem m1.pulse_mem);
-  assert (pm_sep.join m0.pulse_mem m1.pulse_mem == c.pulse_mem);
-  PM.pulse_heap_sig.star_equiv p frame' c.pulse_mem;
+  assert (pm_sep.join m0.pulse_mem m1.pulse_mem == w.pulse_mem);
+  PM.pulse_heap_sig.star_equiv p frame' w.pulse_mem;
   assert (PM.interp (p `PM.star` frame') pulse_mem);
   introduce forall (q:PM.slprop) (m':_).
       PM.interp (q `PM.star` frame') m' ==>
       interpret (lift q `star` frame) { w with pulse_mem=m'}
   with introduce _ ==> _
   with _ . (
-    PM.pulse_heap_sig.star_equiv q frame' (pm_core_of m');
-    eliminate exists (m0' m1':pulse_core_mem).
+    PM.pulse_heap_sig.star_equiv q frame' m';
+    eliminate exists (m0' m1':IndirectionTheorySep.pulse_mem).
         pm_sep.disjoint m0' m1' /\
-        pm_core_of m' == pm_sep.join m0' m1' /\
+        m' == pm_sep.join m0' m1' /\
         PM.pulse_heap_sig.interp q m0' /\
         PM.pulse_heap_sig.interp frame' m1'
     returns _
     with _ . ( 
       assert (fr m1');
-      let mres = core_of { w with pulse_mem = m'} in
-      introduce exists (ml mr:core_mem).
+      let mres = { w with pulse_mem = m'} in
+      introduce exists (ml mr:mem).
         disjoint ml mr /\
         mres == join ml mr /\
         interp (lift q) ml /\
@@ -111,10 +109,10 @@ let pin_frame (p:pm_slprop) (frame:slprop)
         let ml = { pulse_mem=m0'; istore=m0.istore } in
         let mr = { pulse_mem=m1'; istore=m1.istore } in
         assert (pm_sep.disjoint m0' m1');
-        assert (pm_sep.join m0' m1' == pm_core_of m');
+        assert (pm_sep.join m0' m1' == m');
         assert (istore_disjoint m0.istore m1.istore);
-        assert (istore_join m0.istore m1.istore == c.istore);
-        assert (c.istore == mres.istore);
+        assert (istore_join m0.istore m1.istore == w.istore);
+        assert (w.istore == mres.istore);
         assert (interp frame mr);
         lift_eq q;
         assert (interp (lift q) ml)
@@ -215,9 +213,9 @@ let later_intro (e:inames) (p:slprop)
 = fun frame s0 ->
     let open FStar.Ghost in
     sep_laws();
-    let m0, m1 = split_mem p (frame `star` mem_invariant e s0) (core_of s0) in
+    let m0, m1 = split_mem p (frame `star` mem_invariant e s0) s0 in
     intro_later p m0;
-    star_equiv (later p) (frame `star` mem_invariant e s0) (core_of s0);
+    star_equiv (later p) (frame `star` mem_invariant e s0) s0;
     is_ghost_action_refl s0;
     (), s0
 
@@ -226,40 +224,40 @@ let later_elim (e:inames) (p:slprop)
 = fun frame s0 ->
     let open FStar.Ghost in
     sep_laws();
-    let m1, m2, m3 = split_mem3 (later_credit 1) (later p) (frame `star` mem_invariant e s0) (core_of s0) in
+    let m1, m2, m3 = split_mem3 (later_credit 1) (later p) (frame `star` mem_invariant e s0) s0 in
     interp_later_credit 1 m1;
     assert (interp (later_credit 1) m1);
     disjoint_join_levels m2 m3;
     disjoint_join_levels m1 (join m2 m3);
     assert (level m1 > 0 /\ level m2 > 0);
-    let m1' : erased core_mem = age1 m1 in
-    let m2' : erased core_mem = age1 m2 in
+    let m1' : erased mem = age1 m1 in
+    let m2' : erased mem = age1 m2 in
     let m31, m32 = split_mem frame (mem_invariant e s0) m3 in
-    let m31' : erased core_mem = age1 m31 in
+    let m31' : erased mem = age1 m31 in
     age_hereditary frame m31;
-    let m32' : erased core_mem = age1 m32 in
+    let m32' : erased mem = age1 m32 in
     disjoint_join_levels m1 (join m2 m3);
     disjoint_join_levels m2 m3;
     disjoint_join_levels m31 m32;
     assert (level m32 == level m3);
     assert (level m32 == level m1);
-    assert (level m1 == level (core_of s0));
+    assert (level m1 == level s0);
     assert (level m1 > 1);
     mem_invariant_age e s0 m32;
     age_disjoint m31 m32;
     intro_star frame (mem_invariant e (age_mem s0)) m31' m32';
-    let m3' : erased core_mem = age1 m3 in
+    let m3' : erased mem = age1 m3 in
     assert (interp (frame `star` mem_invariant e (age_mem s0)) m3');
     age_later p m2;
     assert (interp p m2');
     age_level m1;
-    assert (level m1' == level (core_of s0) - 1);
+    assert (level m1' == level s0 - 1);
     assert (credits m1' > 0);
-    let m1'' : erased core_mem = spend m1' in
+    let m1'' : erased mem = spend m1' in
     age_disjoint m2 m3;
     age_disjoint m1 (join m2 m3);
     spend_disjoint m1' (join m2' m3');
-    let m : erased core_mem = join m1'' (join m2' m3') in
+    let m : erased mem = join m1'' (join m2' m3') in
     intro_star p (frame `star` mem_invariant e (age_mem s0)) m2' m3';
     emp_equiv m1'';
     intro_star emp (p `star` (frame `star` mem_invariant e (age_mem s0))) m1'' (join m2' m3');
@@ -271,7 +269,7 @@ let later_elim (e:inames) (p:slprop)
     (==) { spend_lemma m1' }
       level m1';
     (==) { }
-      level (core_of s0) - 1;
+      level s0 - 1;
     };
     calc (==) {
       credits m;
@@ -294,12 +292,12 @@ let later_elim (e:inames) (p:slprop)
         }
       credits m1 + credits (join m2 m3) - 1;
     (==) {}
-      credits (core_of s0) - 1;
+      credits s0 - 1;
     };
-    assert (reveal m == spend (age1 (core_of s0)));
+    assert (reveal m == spend (age1 s0));
     let s1 = age_mem s0 in
     let s2 = spend_mem s1 in
-    assert (reveal m == core_of s2);
+    assert (reveal m == s2);
     is_ghost_action_trans s0 s1 s2;
     assert (is_ghost_action s0 s2);
     mem_invariant_spend e s1;
@@ -319,17 +317,17 @@ let buy (e:inames) (n:FStar.Ghost.erased nat)
 : buy_act unit e emp (fun _ -> later_credit n)
 = fun frame s0 ->
     sep_laws();
-    let m0, m1 = split_mem emp (frame `star` mem_invariant e s0) (core_of s0) in
-    let m0' : erased core_mem = buy n m0 in
+    let m0, m1 = split_mem emp (frame `star` mem_invariant e s0) s0 in
+    let m0' : erased mem = buy n m0 in
     buy_lemma n m0;
     interp_later_credit n m0';
     assert (interp (later_credit n) m0');
     buy_disjoint n m0 m1;
     assert (disjoint m0' m1);
     intro_star (later_credit n) (frame `star` mem_invariant e s0) m0' m1;
-    let m' : erased core_mem = join m0' m1 in
+    let m' : erased mem = join m0' m1 in
     let s1 = buy_mem n s0 in
-    assert (reveal m' == core_of s1);
+    assert (reveal m' == s1);
     mem_invariant_buy e n s0;
     inames_ok_update e s0 s1;
     (), s1
@@ -345,7 +343,7 @@ let dup_inv (e:inames) (i:iref) (p:slprop)
     is_ghost_action_refl s0;
     (), s0
 
-let intro_read_inv (i:iref) (p frame:slprop) (m:core_mem)
+let intro_read_inv (i:iref) (p frame:slprop) (m:mem)
 : Lemma
   (requires 
     iname_ok i m /\
@@ -363,7 +361,7 @@ let intro_read_inv (i:iref) (p frame:slprop) (m:core_mem)
   read_inv_disjoint i sl sr;
   intro_star (later (read_inv i m)) (inv i p `star` frame) sl sr
 
-let elim_read_inv (i:iref) (p frame:slprop) (m:core_mem)
+let elim_read_inv (i:iref) (p frame:slprop) (m:mem)
 : Lemma
   (requires 
     iname_ok i m /\
@@ -383,7 +381,7 @@ let elim_read_inv (i:iref) (p frame:slprop) (m:core_mem)
   assert (interp (later p) sl);
   intro_star (later p) (inv i p `star` frame) sl sr
 
-let intro_read_inv_later (i:iref) (p frame:slprop) (m:core_mem)
+let intro_read_inv_later (i:iref) (p frame:slprop) (m:mem)
 : Lemma
   (requires 
     iname_ok i m /\
@@ -402,12 +400,12 @@ let fresh_invariant (e:inames) (p:slprop) (ctx:FStar.Ghost.erased (list iref))
 = fun frame s0 ->
     let (| i, s0' |) = fresh_inv p s0 ctx in
     let s1 = join_mem s0 s0' in
-    disjoint_join_levels (core_of s0) (core_of s0');
+    disjoint_join_levels s0 s0';
     mem_invariant_disjoint e (single i) (p `star` frame) (inv i p) s0 s0';
     assert (interp 
               ((p `star` frame) `star` inv i p `star`
                 (mem_invariant (GhostSet.union e (single i)) s1))
-              (core_of s1));
+              s1);
     sep_laws ();
     assert (GhostSet.union e (single i) `GhostSet.equal` (add_inv e i));
     inames_ok_istore_dom e s0;
@@ -416,26 +414,26 @@ let fresh_invariant (e:inames) (p:slprop) (ctx:FStar.Ghost.erased (list iref))
     assert (interp 
               (inv i p `star`
               (frame `star` p `star` mem_invariant (add_inv e i) s1))
-              (core_of s1));
+              s1);
     destruct_star_l (inv i p)
                     (frame `star` p `star` mem_invariant (add_inv e i) s1)
-                    (core_of s1);
-    inames_ok_single i p (core_of s1);
-    assert (iname_ok i (core_of s1));
-    intro_read_inv_later i p (frame `star` mem_invariant (add_inv e i) s1) (core_of s1);
+                    s1;
+    inames_ok_single i p s1;
+    assert (iname_ok i s1);
+    intro_read_inv_later i p (frame `star` mem_invariant (add_inv e i) s1) s1;
     assert (interp (inv i p `star`
                     frame `star`
                     (mem_invariant (add_inv e i) s1 `star`
-                    later (read_inv i (core_of s1)))) (core_of s1));
+                    later (read_inv i s1))) s1);
     mem_invariant_equiv e s1 i;
-    assert (interp (inv i p `star` frame `star` mem_invariant e s1) (core_of s1));    
+    assert (interp (inv i p `star` frame `star` mem_invariant e s1) s1);    
     assert (is_ghost_action s0 s1);
     inames_ok_disjoint e (single i) s0 s0';
     inames_ok_union e (single i) s1;
     assert (inames_ok e s1);
     assert (is_full s1);
-    disjoint_join_levels (core_of s0) (core_of s0');
-    assert (level (core_of s0) == level (core_of s0'));
+    disjoint_join_levels s0 s0';
+    assert (level s0 == level s0');
     assert (level_decreases_by_spent_credits s0 s1);
     i, s1
 
@@ -443,7 +441,7 @@ let new_invariant (e:inames) (p:slprop)
 : ghost_act iref e p (fun i -> inv i p)
 = fresh_invariant e p []
 
-let iname_ok_frame (i:iref) (p:slprop) (frame:slprop) (m:core_mem)
+let iname_ok_frame (i:iref) (p:slprop) (frame:slprop) (m:mem)
 : Lemma
   (requires interp (inv i p `star` frame) m)
   (ensures iname_ok i m)
@@ -466,33 +464,33 @@ let with_invariant (#a:Type)
       (fun x -> inv i p `star` fp' x)
 = fun frame s0 ->
     sep_laws();
-    iname_ok_frame i p (fp `star` frame `star` mem_invariant opened_invariants s0) (core_of s0);
-    assert (iname_ok i (core_of s0));
+    iname_ok_frame i p (fp `star` frame `star` mem_invariant opened_invariants s0) s0;
+    assert (iname_ok i s0);
     assert (inames_ok (single i) s0);
     mem_invariant_equiv opened_invariants s0 i;
     assert (interp (inv i p `star` fp `star` frame `star` 
-              (mem_invariant (add_inv opened_invariants i) s0 `star` later (read_inv i (core_of s0)))) (core_of s0));
-    elim_read_inv i p (fp `star` frame `star` mem_invariant (add_inv opened_invariants i) s0) (core_of s0);
+              (mem_invariant (add_inv opened_invariants i) s0 `star` later (read_inv i s0))) s0);
+    elim_read_inv i p (fp `star` frame `star` mem_invariant (add_inv opened_invariants i) s0) s0;
     inames_ok_union (single i) opened_invariants s0;
     assert (inames_ok (add_inv opened_invariants i) s0);
     assert (interp ((later p `star` fp) 
                     `star` (frame `star` inv i p)
                     `star` mem_invariant (add_inv opened_invariants i) s0)
-                    (core_of s0));
+                    s0);
     let x, s1 = f (frame `star` inv i p) s0 in
     inames_ok_union (single i) opened_invariants s1;
     assert (inames_ok (single i) s1);
-    assert (iname_ok i (core_of s1));
-    intro_read_inv i p (fp' x `star` frame `star` mem_invariant (add_inv opened_invariants i) s1) (core_of s1);
+    assert (iname_ok i s1);
+    intro_read_inv i p (fp' x `star` frame `star` mem_invariant (add_inv opened_invariants i) s1) s1;
     assert (interp ((inv i p `star` fp' x) 
                     `star` frame
-                    `star` (mem_invariant (add_inv opened_invariants i) s1 `star` later (read_inv i (core_of s1))))
-                    (core_of s1));
+                    `star` (mem_invariant (add_inv opened_invariants i) s1 `star` later (read_inv i s1)))
+                    s1);
     mem_invariant_equiv opened_invariants s1 i;
     assert (interp ((inv i p `star` fp' x) 
                     `star` frame
                     `star` mem_invariant opened_invariants s1)
-                    (core_of s1));
+                    s1);
     inames_ok_union (single i) opened_invariants s1;
     x, s1
 
@@ -504,7 +502,7 @@ let invariant_name_identifies_invariant e i p q
     let m0, m1 =
         split_mem (inv i p `star` inv i q)
                   (inv i p `star` inv i q `star` frame `star` mem_invariant e s0)
-                  (core_of s0)
+                  s0
     in
     disjoint_join_levels m0 m1;
     invariant_name_identifies_invariant i p q m0;
@@ -530,12 +528,12 @@ let witness_exists (#opened_invariants:_) (#a:_) (p:a -> slprop)
            (fun x -> p x)
 = fun frame s0 ->
     sep_laws();
-    let m1, m2 = split_mem (op_exists_Star p) (frame `star` mem_invariant opened_invariants s0) (core_of s0) in 
+    let m1, m2 = split_mem (op_exists_Star p) (frame `star` mem_invariant opened_invariants s0) s0 in 
     interp_exists p;
     eliminate exists x. interp (p x) m1
-    returns exists x. interp (p x `star` (frame `star` mem_invariant opened_invariants s0)) (core_of s0)
+    returns exists x. interp (p x `star` (frame `star` mem_invariant opened_invariants s0)) s0
     with _. (
-        star_equiv (p x) (frame `star` mem_invariant opened_invariants s0) (core_of s0)
+        star_equiv (p x) (frame `star` mem_invariant opened_invariants s0) s0
     );
     let x =
       FStar.IndefiniteDescription.indefinite_description_tot
@@ -551,9 +549,9 @@ let intro_exists (#opened_invariants:_) (#a:_) (p:a -> slprop) (x:erased a)
   (fun _ -> op_exists_Star p)
 = fun frame s0 ->
     sep_laws();
-    let m1, m2 = split_mem (p x) (frame `star` mem_invariant opened_invariants s0) (core_of s0) in
+    let m1, m2 = split_mem (p x) (frame `star` mem_invariant opened_invariants s0) s0 in
     interp_exists p;
-    star_equiv (op_exists_Star p) (frame `star` mem_invariant opened_invariants s0) (core_of s0);
+    star_equiv (op_exists_Star p) (frame `star` mem_invariant opened_invariants s0) s0;
     is_ghost_action_refl s0;
     (), s0
 
@@ -564,21 +562,21 @@ let raise_exists (#opened_invariants:_) (#a:Type u#a) (p:a -> slprop)
 = fun frame s0 ->
     let x, s1 = witness_exists #opened_invariants #a p frame s0 in
     sep_laws();
-    let m1, m2 = split_mem (p x) (frame `star` mem_invariant opened_invariants s1) (core_of s1) in
+    let m1, m2 = split_mem (p x) (frame `star` mem_invariant opened_invariants s1) s1 in
     assert (interp ((U.lift_dom p) (U.raise_val u#a u#b (reveal x))) m1);
     interp_exists (U.lift_dom u#a u#_ u#b p);
     assert (interp (op_exists_Star #(U.raise_t u#a u#b a) (U.lift_dom p)) m1);
-    star_equiv (op_exists_Star #(U.raise_t u#a u#b a) (U.lift_dom p)) (frame `star` mem_invariant opened_invariants s1) (core_of s1);
+    star_equiv (op_exists_Star #(U.raise_t u#a u#b a) (U.lift_dom p)) (frame `star` mem_invariant opened_invariants s1) s1;
     (), s1
 
 let elim_pure (#opened_invariants:_) (p:prop)
 : ghost_act (u:unit{p}) opened_invariants (pure p) (fun _ -> emp)
 = fun frame s0 ->
     sep_laws();
-    let m1, m2 = split_mem (pure p) (frame `star` mem_invariant opened_invariants s0) (core_of s0) in
+    let m1, m2 = split_mem (pure p) (frame `star` mem_invariant opened_invariants s0) s0 in
     interp_pure p m1;
     emp_equiv m1;
-    star_equiv emp (frame `star` mem_invariant opened_invariants s0) (core_of s0);
+    star_equiv emp (frame `star` mem_invariant opened_invariants s0) s0;
     is_ghost_action_refl s0;
     (), s0
 
@@ -586,9 +584,9 @@ let intro_pure (#opened_invariants:_) (p:prop) (_:squash p)
 : ghost_act unit opened_invariants emp (fun _ -> pure p)
 = fun frame s0 -> 
     sep_laws();
-    let m1, m2 = split_mem emp (frame `star` mem_invariant opened_invariants s0) (core_of s0) in
+    let m1, m2 = split_mem emp (frame `star` mem_invariant opened_invariants s0) s0 in
     interp_pure p m1;
-    star_equiv (pure p) (frame `star` mem_invariant opened_invariants s0) (core_of s0);
+    star_equiv (pure p) (frame `star` mem_invariant opened_invariants s0) s0;
     is_ghost_action_refl s0;
     (), s0
 
@@ -596,9 +594,9 @@ let drop (#opened_invariants:_) (p:slprop)
 : ghost_act unit opened_invariants p (fun _ -> emp)
 = fun frame s0 -> 
     sep_laws();
-    let m1, m2 = split_mem p (frame `star` mem_invariant opened_invariants s0) (core_of s0) in
+    let m1, m2 = split_mem p (frame `star` mem_invariant opened_invariants s0) s0 in
     emp_equiv m1;
-    star_equiv emp (frame `star` mem_invariant opened_invariants s0) (core_of s0);
+    star_equiv emp (frame `star` mem_invariant opened_invariants s0) s0;
     is_ghost_action_refl s0;
     (), s0
 
