pulse/lib/pulse/core/PulseCore.IndirectionTheoryActions.fsti
@@ -9,7 +9,7 @@ type action_kind =
 | ATOMIC
 | BUY
 let maybe_ghost_action (k:action_kind) (m0 m1:mem) = GHOST? k ==> is_ghost_action m0 m1
-let interpret (p:slprop) (m:mem) = interp p (core_of m)
+let interpret (p:slprop) (m:mem) = interp p m
 let _ACTION 
   (a:Type u#a)
   (ak:action_kind)
